zoo_std/ivar_{1,2,3}: Add [is_unset].

lib/zoo_std/ivar_1.ml
@@ -13,8 +13,10 @@ let make v =
 let try_get t =
   Atomic.get t
 
+let is_unset t =
+  try_get t == None
 let is_set t =
-  try_get t != None
+  not @@ is_unset t
 
 let get t =
   match try_get t with
