theories/zoo_std/ivar_1__opaque.v
@@ -3,6 +3,7 @@ From zoo_std Require Import
 
 #[global] Opaque ivar_1_create.
 #[global] Opaque ivar_1_make.
+#[global] Opaque ivar_1_is_unset.
 #[global] Opaque ivar_1_is_set.
 #[global] Opaque ivar_1_try_get.
 #[global] Opaque ivar_1_get.
