theories/zoo_std/ivar_2__opaque.v
@@ -3,6 +3,7 @@ From zoo_std Require Import
 
 #[global] Opaque ivar_2_create.
 #[global] Opaque ivar_2_make.
+#[global] Opaque ivar_2_is_unset.
 #[global] Opaque ivar_2_is_set.
 #[global] Opaque ivar_2_try_get.
 #[global] Opaque ivar_2_get.
