theories/zoo_std/ivar_3__opaque.v
@@ -3,6 +3,7 @@ From zoo_std Require Import
 
 #[global] Opaque ivar_3_create.
 #[global] Opaque ivar_3_make.
+#[global] Opaque ivar_3_is_unset.
 #[global] Opaque ivar_3_is_set.
 #[global] Opaque ivar_3_try_get.
 #[global] Opaque ivar_3_get.
